Try start llist_set_succ

pulse/examples/steel/arraystructs/LList.fst
@@ -78,7 +78,7 @@ let pts_to_llist_cons (value: int) (next: ptr) (tl: cells)
   (r `pts_to` mk_node (some value) (some next)) `star`
   (next `pts_to_llist` Ghost.hide tl)
 
-let rec pts_to_llist ([@@@smt_fallback] p:ptr) ([@@@smt_fallback] l:Ghost.erased cells)
+let rec pts_to_llist (p:ptr) ([@@@smt_fallback] l:Ghost.erased cells)
 : Tot vprop (decreases (List.length l))
 = match Ghost.reveal l with
   | [] -> vpure (p == None)
@@ -101,7 +101,6 @@ let pts_to_llist_cons_eq (p:ptr) (value:int) (next:ptr) (tl:cells)
   | (value, next) :: tl ->
     vpure (Some? p /\ pcm_of_ref' (Some?.v p) == node_pcm) `vdep`
     pts_to_llist_cons value next tl pts_to_llist p)) 
-    // TODO Why do I have to keep the match around?
 
 let pts_to_llist_cons_eq' (p: ptr) value (next:ptr) tl prf
 : Lemma (pts_to_llist_cons value next tl pts_to_llist p prf ==
@@ -193,11 +192,12 @@ let cells_set_hd x (l: cells) = match l with
   | [] -> []
   | (_, next) :: l' -> (x, next) :: l'
 
-/// Mutate the head of a list
+val exfalso (#opened:inames) (p q:vprop) (r:prop)
+: SteelGhostF unit opened p (fun _ -> q) (requires fun _ -> False) (ensures fun _ _ _ -> r)
 
-// TODO does this exist already?
-assume val exfalso (#opened:inames) (p:vprop) (q:prop)
-: SteelGhost unit opened emp (fun _ -> p) (requires fun _ -> False) (ensures fun _ _ _ -> q)
+let exfalso (#opened:inames) (p q:vprop) (r:prop)
+: SteelGhostF unit opened p (fun _ -> q) (requires fun _ -> False) (ensures fun _ _ _ -> r)
+= change_slprop_rel p q (fun _ _ -> r) (fun _ -> ())
 
 val pts_to_llist_nullptr (#opened:inames) (p:ptr) (l:Ghost.erased cells)
 : SteelGhost unit opened
@@ -213,8 +213,7 @@ let pts_to_llist_nullptr p l =
     change_equal_slprop (p `pts_to_llist` l) (None `pts_to_llist` ((value, next) :: tl));
     let r = elim_llist_cons None value next tl in
     assert (None == Some r);
-    sladmit() // TODO
-    //exfalso (None `pts_to_llist` []) (Ghost.reveal l == [])
+    exfalso _ _ (Ghost.reveal l == [])
 
 [@@erasable]
 noeq type pts_to_llist_res = {
@@ -237,20 +236,87 @@ let pts_to_llist_some p l =
   | [] ->
     change_equal_slprop (p `pts_to_llist` l) (p `pts_to_llist` []);
     assert (Some? p /\ p == None);
-    sladmit() // TODO
+    exfalso _ _ 
+      (Some? p /\ pcm_of_ref' (Some?.v p) == node_pcm /\
+       Ghost.reveal l == ((res.value, res.next) :: res.tl))
   | (value, next) :: tl ->
     change_equal_slprop (p `pts_to_llist` l) (p `pts_to_llist` ((value, next) :: tl));
     {value; next; tl}
 
-val set_hd (p:ptr) (l:cells) (value:int)
+val set_hd (p:ptr) (l:Ghost.erased cells) (value:int)
 : SteelT unit
     (p `pts_to_llist` l)
     (fun _ -> p `pts_to_llist` cells_set_hd value l)
 
 let set_hd p l new_value =
   match p with
-  | None -> pts_to_llist_nullptr p l; return ()
+  | None -> 
+    pts_to_llist_nullptr p l;
+    change_equal_slprop (None `pts_to_llist` []) (p `pts_to_llist` []);
+    return ()
   | Some r ->
+    let res = pts_to_llist_some p l in
+    let value: Ghost.erased int = Ghost.hide res.value in
+    let next: Ghost.erased ptr = Ghost.hide res.next in
+    let tl: Ghost.erased cells = Ghost.hide res.tl in
+    //let value: Ghost.erased int = Ghost.hide (fst value_next_tl) in
+    //let next: Ghost.erased ptr = Ghost.hide (fst (snd value_next_tl)) in
+    //let tl: Ghost.erased cells = Ghost.hide (snd (snd value_next_tl)) in
+    change_equal_slprop (p `pts_to_llist` l)
+      (Some r `pts_to_llist` _);
+       //Ghost.hide ((Ghost.reveal value, Ghost.reveal next) :: Ghost.reveal tl));
+    let r' = elim_llist_cons (Some r) (Ghost.reveal value) (Ghost.reveal next) (Ghost.reveal tl) in
+    let r: ref node node_pcm = r in
+    //assert (Ghost.reveal r' == r);
+    //slassert (Ghost.reveal r' `pts_to` mk_node (some value) (some next));
+    change_equal_slprop (Ghost.reveal r' `pts_to` mk_node (some value) (some next))
+      (r `pts_to` mk_node (some value) (some next));
+    let r_value = addr_of_value r in
+    r_value `opt_write` new_value;
+    unaddr_of_value r r_value;
+    intro_llist_cons r new_value next tl;
+    change_equal_slprop (Some r `pts_to_llist` _) (p `pts_to_llist` _);
+    //sladmit(); return ()
+    return ()
+
+// TODO try not to constrain postresources (e.g. in _nullptr; e.g. in intro_llist_cons, take extra p and precondition Some r == p)
+// for the presentation, write write code for set_hd
+// based on assume val for needed selectors, then solve assumes
+
+let rec cells_set_nth (n:nat) (value:int) (l:cells) : Tot cells (decreases n) =
+  if n = 0 then cells_set_hd value l
+  else match l with
+  | [] -> []
+  | hd :: tl -> hd :: cells_set_nth (n - 1) value tl
+
+let rec cells_set_nth_nil n value
+: Lemma (ensures cells_set_nth n value [] == []) (decreases n)
+= if n = 0 then () else cells_set_nth_nil (n - 1) value
+
+let llist_setter (n:nat) =
+  p:ptr -> l:Ghost.erased cells -> value:int ->
+  SteelT unit
+    (p `pts_to_llist` l)
+    (fun _ -> p `pts_to_llist` cells_set_nth n value l)
+
+let llist_set_zero: llist_setter 0 = set_hd
+
+(*
+let aux n (ih: llist_setter n) (p: ptr) (l: Ghost.erased cells) (new_value: int)
+: SteelT unit
+    (p `pts_to_llist` l)
+    (fun _ -> p `pts_to_llist` cells_set_nth (n + 1) new_value l)
+= assume (Some? p);
+  // match p with
+  // | None ->
+  //   pts_to_llist_nullptr p l;
+  //   cells_set_nth_nil (n + 1) value;
+  //   change_equal_slprop
+  //     (None `pts_to_llist` [])
+  //     (p `pts_to_llist` cells_set_nth (n + 1) value l);
+  //   return ()
+  // | Some r ->
+  let Some r = p in
     let res = pts_to_llist_some p l in
     let value: Ghost.erased int = Ghost.hide res.value in
     let next: Ghost.erased ptr = Ghost.hide res.next in
@@ -263,17 +329,84 @@ let set_hd p l new_value =
        Ghost.hide ((Ghost.reveal value, Ghost.reveal next) :: Ghost.reveal tl));
     let r' = elim_llist_cons (Some r) (Ghost.reveal value) (Ghost.reveal next) (Ghost.reveal tl) in
     let r: ref node node_pcm = r in
-    //assert (Ghost.reveal r' == r);
-    //slassert (Ghost.reveal r' `pts_to` mk_node (some value) (some next));
     change_equal_slprop (Ghost.reveal r' `pts_to` mk_node (some value) (some next))
       (r `pts_to` mk_node (some value) (some next));
-    let r_value = addr_of_value r in
-    r_value `opt_write` new_value;
-    unaddr_of_value r r_value;
-    intro_llist_cons r new_value next tl;
-    //change_equal_slprop (Ghost.reveal r' `pts_to` mk_node _ _) (r `pts_to` mk_node _ _);
-    //sladmit(); return ()
-    return ()
+    let r_next = addr_of_next r in
+    let q: ptr = opt_read r_next in
+    assert (q == Ghost.reveal next);
+    unaddr_of_next r r_next;
+    change_equal_slprop (Ghost.reveal next `pts_to_llist` _) (q `pts_to_llist` _);
+    ih q tl new_value;
+    change_equal_slprop (q `pts_to_llist` _) (Ghost.reveal next `pts_to_llist` _);
+    intro_llist_cons r (Ghost.reveal value) (Ghost.reveal next) _;
+//val intro_llist_cons
+//  (#opened:inames) (r: ref node node_pcm)
+//  (value: int) (next: ptr)
+//  (tl: cells)
+//: SteelGhostT unit opened
+//    ((r `pts_to` mk_node (some value) (some next)) `star` (next `pts_to_llist` tl))
+//    (fun _ -> Some r `pts_to_llist` ((value, next)::tl))
+    sladmit(); return ()
+    // //assert (Ghost.reveal r' == r);
+    // //slassert (Ghost.reveal r' `pts_to` mk_node (some value) (some next));
+    // let r_value = addr_of_value r in
+    // r_value `opt_write` new_value;
+    // unaddr_of_value r r_value;
+    // intro_llist_cons r new_value next tl;
+    // //change_equal_slprop (Ghost.reveal r' `pts_to` mk_node _ _) (r `pts_to` mk_node _ _);
+    // //sladmit(); return ()
+    // return ()
+
+let llist_set_succ n (ih: llist_setter n): llist_setter (n + 1) =
+  let aux (p: ptr) (l: Ghost.erased cells) (value: int)
+  : SteelT unit
+      (p `pts_to_llist` l)
+      (fun _ -> p `pts_to_llist` cells_set_nth (n + 1) value l)
+  = assume (Some? p);
+    // match p with
+    // | None ->
+    //   pts_to_llist_nullptr p l;
+    //   cells_set_nth_nil (n + 1) value;
+    //   change_equal_slprop
+    //     (None `pts_to_llist` [])
+    //     (p `pts_to_llist` cells_set_nth (n + 1) value l);
+    //   return ()
+    // | Some r ->
+    let Some r = p in
+      let res = pts_to_llist_some p l in
+      let value: Ghost.erased int = Ghost.hide res.value in
+      let next: Ghost.erased ptr = Ghost.hide res.next in
+      let tl: Ghost.erased cells = Ghost.hide res.tl in
+      //let value: Ghost.erased int = Ghost.hide (fst value_next_tl) in
+      //let next: Ghost.erased ptr = Ghost.hide (fst (snd value_next_tl)) in
+      //let tl: Ghost.erased cells = Ghost.hide (snd (snd value_next_tl)) in
+      change_equal_slprop (p `pts_to_llist` l)
+        (Some r `pts_to_llist`
+         Ghost.hide ((Ghost.reveal value, Ghost.reveal next) :: Ghost.reveal tl));
+      let r' = elim_llist_cons (Some r) (Ghost.reveal value) (Ghost.reveal next) (Ghost.reveal tl) in
+      let r: ref node node_pcm = r in
+      change_equal_slprop (Ghost.reveal r' `pts_to` mk_node (some value) (some next))
+        (r `pts_to` mk_node (some value) (some next));
+      let r_next = addr_of_next r in
+      let q: ptr = opt_read r_next in
+      unaddr_of_next r r_next;
+      //ih q tl value;
+      sladmit(); return ()
+      // //assert (Ghost.reveal r' == r);
+      // //slassert (Ghost.reveal r' `pts_to` mk_node (some value) (some next));
+      // let r_value = addr_of_value r in
+      // r_value `opt_write` new_value;
+      // unaddr_of_value r r_value;
+      // intro_llist_cons r new_value next tl;
+      // //change_equal_slprop (Ghost.reveal r' `pts_to` mk_node _ _) (r `pts_to` mk_node _ _);
+      // //sladmit(); return ()
+      // return ()
+  in aux
+
+*)
+
+// TODO look at #2319, construct module of (possibly null) pointers
+// (define pts_to_or_null; can compare against null only if points to non-unit)
 
 // Mutate the kth element of a list (of fixed k)
 // 
